Adjust request/confidential message postconditions (#101)
* Some small cleanup of EoL spaces

* Revised confidential message/request receipt postconditions

* Cleaned up some invariants and proofs with help of a small utility function

---------

Co-authored-by: Klaas Pruiksma <klaas.pruiksma@sec.uni-stuttgart.de>

src/lib/communication/DY.Lib.Communication.Core.Properties.fst
@@ -8,6 +8,7 @@ open DY.Lib.Event.Typed
 open DY.Lib.State.PKI
 open DY.Lib.State.PrivateKeys
 open DY.Lib.State.Typed
+open DY.Lib.Comparse.DYUtils
 
 open DY.Lib.Communication.Core
 open DY.Lib.Communication.Core.Invariants
@@ -17,6 +18,52 @@ open DY.Lib.Communication.Core.Lemmas
 
 /// This module contains security properties that can be proven from the
 /// communication layer guarantees.
+
+(*** Confidential Messages Properties ***)
+
+val conf_message_secrecy:
+  {|protocol_invariants|} ->
+  #a:Type -> {| parseable_serializeable bytes a |} ->
+  tr:trace -> i:timestamp ->
+  higher_layer_preds:comm_higher_layer_event_preds a ->
+  receiver:principal ->
+  payload:bytes ->
+  Lemma
+  (requires
+    trace_invariant tr /\
+    has_communication_layer_event_predicates higher_layer_preds /\
+    event_triggered_at tr i receiver (CommConfReceiveMsg receiver payload)
+  )
+  (ensures
+    is_knowable_by (principal_label receiver) (prefix tr i) payload /\
+
+    parse_and_pred (fun payload_parsed ->
+      (exists sender. higher_layer_preds.send_conf (prefix tr i) sender receiver payload_parsed) \/
+      is_well_formed a (is_publishable (prefix tr i)) payload_parsed
+    ) payload
+  )
+let conf_message_secrecy #invs #a tr i higher_layer_preds receiver payload =
+  let send_event sender = CommConfSendMsg sender receiver payload in
+  let tr_i = prefix tr i in
+  eliminate (exists sender. event_triggered tr_i sender (send_event sender)) \/
+            is_publishable tr_i payload
+  returns
+    is_knowable_by (principal_label receiver) tr_i payload /\
+    parse_and_pred (fun payload_parsed ->
+      (exists sender. higher_layer_preds.send_conf (prefix tr i) sender receiver payload_parsed) \/
+      is_well_formed a (is_publishable (prefix tr i)) payload_parsed
+    ) payload
+  with _. eliminate exists sender. event_triggered tr_i sender (send_event sender)
+    returns _
+    with _. (
+      let j = find_event_triggered_at_timestamp tr sender (send_event sender) in
+      find_event_triggered_at_timestamp_later tr_i tr sender (send_event sender);
+
+      serialize_parse_inv_lemma a payload;
+      higher_layer_preds.send_conf_later (prefix tr j) tr_i sender receiver (Some?.v (parse a payload))
+    )
+  and _. parse_wf_lemma a (is_publishable (prefix tr i)) payload
+
 
 (*** Authenticated Messages Properties ***)
 
